Splinter/BlockLayer/BlockCoordinationSystemRefinement.i.dfy
@@ -1,101 +1,137 @@
 // Copyright 2018-2021 VMware, Inc., Microsoft Inc., Carnegie Mellon University, ETH Zurich, and University of Washington
 // SPDX-License-Identifier: BSD-2-Clause
 
-include "BlockCoordinationSystem.i.dfy"
+include "../../Spec/MapSpec.s.dfy"
 include "../CoordinationLayer/CoordinationSystem.i.dfy"
+include "../Journal/MarshalledJournalRefinement.i.dfy"
+include "BlockCoordinationSystem.i.dfy"
 
 module BlockCoordinationSystemRefinement
 {
   import opened Options
-  import opened BlockCoordinationSystem
-  import MarshalledJournal
   import CoordinationSystem
-  import AbstractJournal
   import opened MsgHistoryMod
+  import opened ValueMessage
+  import opened BlockCoordinationSystem
+  import AbstractJournal
+  import PagedJournalRefinement
   import LinkedJournal
+  import LinkedJournalRefinement
+  import MarshalledJournalRefinement
 
-  predicate JournalImageInv(journalImage: MarshalledJournal.JournalImage)
+  // Decodable is a pretty cheap almost-type property, but not one we can
+  // trivially check, either with a typecheck in the implementation or a cheap
+  // runtime check, so we don't want to call it WF and risk it ending up in a
+  // v' where it'll be hard to prove later. Instead, we define it here and
+  // prove it as part of Inv.
+  predicate DecodableJournalImage(journalImage: MarshalledJournal.JournalImage)
   {
     && journalImage.WF()
-    && journalImage.I().diskView.Acyclic()
-    && journalImage.I().I().WF()
+    && journalImage.I().Decodable()
   }
 
-  predicate DiskImageInv(diskImage: DiskImage)
+  predicate DecodableDiskImage(diskImage: DiskImage)
   {
-    && JournalImageInv(diskImage.journal)
+    && DecodableJournalImage(diskImage.journal)
   }
 
-  predicate MarshalledJournalInv(v: MarshalledJournal.Variables)
+  predicate DecodableEphemeral(ephemeral: Ephemeral)
   {
-    && JournalImageInv(v.journalImage)
-    && v.unmarshalledTail.WF()
-    && JournalImageI(v.journalImage).CanConcat(v.unmarshalledTail)
+    ephemeral.Known? ==> MarshalledJournalRefinement.Inv(ephemeral.journal)
   }
 
-  predicate EphemeralInv(ephemeral: Ephemeral)
+  predicate DecodableVariables(v: Variables)
   {
-    && (ephemeral.Known? ==> MarshalledJournalInv(ephemeral.journal))
+    && DecodableDiskImage(v.persistentImage)
+    && DecodableEphemeral(v.ephemeral)
+    && (v.inFlightImage.Some? ==> DecodableDiskImage(v.inFlightImage.value))
   }
 
-  predicate Inv(v: Variables)
+  predicate DecodableStep(step: Step)
   {
-    && DiskImageInv(v.persistentImage)
-    && EphemeralInv(v.ephemeral)
-    && (v.inFlightImage.Some? ==> DiskImageInv(v.inFlightImage.value))
+    step.CommitStartStep? ==> DecodableJournalImage(step.frozenJournal)
   }
 
-  function JournalImageI(journalImage: MarshalledJournal.JournalImage) : MsgHistory
-    requires JournalImageInv(journalImage)
+  //////////////////////////////////////////////////////////////////////
+  // Inv
+
+  predicate Inv(v: Variables) {
+    && DecodableVariables(v)
+  }
+
+  // IA Interpret to Abstraction: peel all the way up the stack.
+  function IAJournalImage(journalImage: MarshalledJournal.JournalImage) : MsgHistory
+    requires DecodableJournalImage(journalImage)
   {
     journalImage.I().I().I()
   }
 
-  function DiskImageI(diskImage: DiskImage) : CoordinationSystem.DiskImage
-    requires DiskImageInv(diskImage)
+  function IAJournal(journal: MarshalledJournal.Variables) : AbstractJournal.Variables
+    requires MarshalledJournalRefinement.Inv(journal)
   {
-    CoordinationSystem.DiskImage(diskImage.mapadt, JournalImageI(diskImage.journal))
+    PagedJournalRefinement.I(LinkedJournalRefinement.I(MarshalledJournalRefinement.I(journal)))
   }
 
-  function MarshalledJournalI(v: MarshalledJournal.Variables) : AbstractJournal.Variables
-    requires MarshalledJournalInv(v)
+  // Interpret BlockCoordinationSystem types
+  function IDiskImage(diskImage: DiskImage) : CoordinationSystem.DiskImage
+    requires DecodableDiskImage(diskImage)
   {
-    AbstractJournal.Variables(JournalImageI(v.journalImage).Concat(v.unmarshalledTail))
+    CoordinationSystem.DiskImage(diskImage.mapadt, IAJournalImage(diskImage.journal))
   }
 
-  function EphemeralI(ephemeral: Ephemeral) : CoordinationSystem.Ephemeral
-    requires EphemeralInv(ephemeral)
+  function IEphemeral(ephemeral: Ephemeral) : CoordinationSystem.Ephemeral
+    requires DecodableEphemeral(ephemeral)
   {
-    if ephemeral.Unknown? then
-      CoordinationSystem.Unknown
-    else
-      CoordinationSystem.Known(
+    if ephemeral.Unknown? then CoordinationSystem.Unknown
+    else CoordinationSystem.Known(
       ephemeral.progress,
       ephemeral.syncReqs,
       ephemeral.mapadt,
       ephemeral.mapLsn,
-      MarshalledJournalI(ephemeral.journal),
+      IAJournal(ephemeral.journal),
       ephemeral.frozenMap
-      )
+    )
   }
 
   function I(v: Variables) : CoordinationSystem.Variables
-    requires Inv(v)
+    requires DecodableVariables(v)
   {
     CoordinationSystem.Variables(
-      DiskImageI(v.persistentImage),
-      EphemeralI(v.ephemeral),
-      if v.inFlightImage.Some? then Some(DiskImageI(v.inFlightImage.value)) else None
-      )
+      IDiskImage(v.persistentImage),
+      IEphemeral(v.ephemeral),
+      if v.inFlightImage.None? then None else Some(IDiskImage(v.inFlightImage.value))
+    )
+  }
+  
+  lemma RefinementInit(v: Variables)
+    requires Init(v)
+    ensures Inv(v)
+    ensures CoordinationSystem.Init(I(v))
+  {
+    MarshalledJournalRefinement.MkfsRefines();
+    assert MarshalledJournal.Mkfs().WF();
+    assert DecodableDiskImage(v.persistentImage);
+    assert DecodableVariables(v);
   }
 
-  lemma RefinementInit(v: Variables)
-    requires v.Init()
-    ensures Inv(v)
-    ensures I(v).Init()
+  function IStep(step: Step) : CoordinationSystem.Step
+    requires DecodableStep(step)
   {
-    assert v.persistentImage.journal.TypeProvidesModel(LinkedJournal.Mkfs());
-    assert v.persistentImage.journal.I().diskView.PointersRespectRank(map[]);
+    match step
+      case LoadEphemeralFromPersistentStep() => CoordinationSystem.LoadEphemeralFromPersistentStep
+      case RecoverStep(puts) => CoordinationSystem.RecoverStep(puts)
+      case AcceptRequestStep() => CoordinationSystem.AcceptRequestStep()
+      case QueryStep() => CoordinationSystem.QueryStep()
+      case PutStep() => CoordinationSystem.PutStep()
+      case DeliverReplyStep() => CoordinationSystem.DeliverReplyStep
+//    case | JournalInternalStep() => CoordinationSystem.JournalInternalStep()
+//    case | SplinterTreeInternalStep() => CoordinationSystem.SplinterTreeInternalStep()
+      case ReqSyncStep() => CoordinationSystem.ReqSyncStep
+      case ReplySyncStep() => CoordinationSystem.ReplySyncStep
+      case FreezeMapAdtStep() => CoordinationSystem.FreezeMapAdtStep
+      case CommitStartStep(seqBoundary, frozenJournal) => CoordinationSystem.CommitStartStep(IAJournalImage(frozenJournal))
+      case CommitCompleteStep() => CoordinationSystem.CommitCompleteStep()
+      case CrashStep() => CoordinationSystem.CrashStep()
   }
 
   lemma RefinementNext(v: Variables, v': Variables, uiop: UIOp)
@@ -103,4 +139,81 @@ module BlockCoordinationSystemRefinement
     requires Next(v, v', uiop)
     ensures Inv(v')
     ensures CoordinationSystem.Next(I(v), I(v'), uiop)
+  {
+    var step :| NextStep(v, v', uiop, step);
+    match step {
+      case LoadEphemeralFromPersistentStep() => {
+        MarshalledJournalRefinement.InvInit(v'.ephemeral.journal, v.persistentImage.journal);
+        assert Inv(v'); // case boilerplate
+
+        var j := v.persistentImage.journal;
+        var j' := v'.ephemeral.journal;
+
+        assert MarshalledJournal.Init(j', j);
+        MarshalledJournalRefinement.RefinementInit(j', j);
+        assert LinkedJournal.Init(MarshalledJournalRefinement.I(j'), j.I());
+        
+
+        assert I(v').ephemeral.journal.journal == I(v).persistentImage.journal;
+        assert AbstractJournal.Init(I(v').ephemeral.journal, I(v).persistentImage.journal);
+        assert CoordinationSystem.LoadEphemeralFromPersistent(I(v), I(v'), uiop);
+        assert CoordinationSystem.NextStep(I(v), I(v'), uiop, IStep(step));
+      }
+      case RecoverStep(puts) => {
+        assert Inv(v'); // case boilerplate
+        assert CoordinationSystem.NextStep(I(v), I(v'), uiop, IStep(step));
+      }
+      case AcceptRequestStep() => {
+        assert Inv(v'); // case boilerplate
+        assert CoordinationSystem.NextStep(I(v), I(v'), uiop, IStep(step));
+      }
+      case QueryStep() => {
+        assert Inv(v'); // case boilerplate
+        assert CoordinationSystem.NextStep(I(v), I(v'), uiop, IStep(step));
+      }
+      case PutStep() => {
+        var key := uiop.baseOp.req.input.key;
+        var val := uiop.baseOp.req.input.value;
+        var singleton := MsgHistoryMod.SingletonAt(v.ephemeral.mapLsn, KeyedMessage(key, Define(val)));
+        MarshalledJournalRefinement.RefinementNext(v.ephemeral.journal, v'.ephemeral.journal, MarshalledJournal.PutLabel(singleton));
+      
+        assert Inv(v'); // case boilerplate
+        assert CoordinationSystem.NextStep(I(v), I(v'), uiop, IStep(step));
+      }
+//      case JournalInternalStep(sk) => {
+//}
+//      case SplinterTreeInternalStep(sk) => {
+//}
+      case DeliverReplyStep() => {
+        assert Inv(v'); // case boilerplate
+        assert CoordinationSystem.NextStep(I(v), I(v'), uiop, IStep(step));
+      }
+      case ReqSyncStep() => {
+        assert Inv(v'); // case boilerplate
+        assert CoordinationSystem.NextStep(I(v), I(v'), uiop, IStep(step));
+      }
+      case ReplySyncStep() => {
+        assert Inv(v'); // case boilerplate
+        assert CoordinationSystem.NextStep(I(v), I(v'), uiop, IStep(step));
+      }
+      case FreezeMapAdtStep() => {
+        assert Inv(v'); // case boilerplate
+        assert CoordinationSystem.NextStep(I(v), I(v'), uiop, IStep(step));
+      }
+      case CommitStartStep(seqBoundary, frozenJournal) => {
+        assert Inv(v'); // case boilerplate
+        assert CoordinationSystem.NextStep(I(v), I(v'), uiop, IStep(step));
+      }
+      case CommitCompleteStep() => {
+        MarshalledJournalRefinement.RefinementNext(v.ephemeral.journal, v'.ephemeral.journal,
+          MarshalledJournal.DiscardOldLabel(v.inFlightImage.value.mapadt.seqEnd, v.ephemeral.mapLsn));
+        assert Inv(v'); // case boilerplate
+        assert CoordinationSystem.NextStep(I(v), I(v'), uiop, IStep(step));
+      }
+      case CrashStep() => {
+        assert Inv(v'); // case boilerplate
+        assert CoordinationSystem.NextStep(I(v), I(v'), uiop, IStep(step));
+      }
+    }
+  }
 }
